Define canonical parameter opcode classifier

venom/defs/venomInstScript.sml
@@ -570,6 +570,28 @@ Definition is_raw_fmp_opcode_def:
   is_raw_fmp_opcode _ = F
 End
 
+(* Canonical classification for all parameter-like pseudo instructions. *)
+Definition is_param_opcode_def:
+  is_param_opcode PARAM = T /\
+  is_param_opcode FMP_PARAM = T /\
+  is_param_opcode RETPC_PARAM = T /\
+  is_param_opcode _ = F
+End
+
+Theorem is_param_opcode_iff:
+  is_param_opcode op <=>
+    (op = PARAM \/ op = FMP_PARAM \/ op = RETPC_PARAM)
+Proof
+  Cases_on `op` >> simp[is_param_opcode_def]
+QED
+
+Theorem is_param_opcode_eval:
+  MAP is_param_opcode [PARAM; FMP_PARAM; RETPC_PARAM] = [T; T; T]
+Proof
+  EVAL_TAC
+QED
+
+(* Compatibility classifier for the two hidden physical parameters only. *)
 Definition is_fmp_param_opcode_def:
   is_fmp_param_opcode FMP_PARAM = T /\
   is_fmp_param_opcode RETPC_PARAM = T /\
@@ -707,6 +729,7 @@ Theorem task006_opcode_classification_eval:
   let ops = [DALLOCA; DRET; GETFMP; SETFMP; RETFMP;
              INITIAL_FMP; BUMP; FMP_PARAM; RETPC_PARAM] in
     MAP is_raw_fmp_opcode ops = [T; T; T; T; T; F; F; F; F] /\
+    MAP is_param_opcode [PARAM; FMP_PARAM; RETPC_PARAM] = [T; T; T] /\
     MAP is_fmp_param_opcode ops = [F; F; F; F; F; F; F; T; T] /\
     MAP is_terminator ops = [F; T; F; F; T; F; F; F; F] /\
     MAP is_pseudo ops = [F; F; F; F; F; F; F; T; T] /\
